update Zulib

src/Zulib/fsharp/Realized/Zen.Set.fs
@@ -1,0 +1,30 @@
+module Zen.Set
+
+module Cost = Zen.Cost.Realized
+
+type set<'a when 'a : comparison> =
+    // A set, plus the number of elements in the set
+    Set<'a> * uint32
+
+type t<'a when 'a : comparison> = set<'a>
+
+let nullSet : set<'a> = Set.empty, 0u
+
+let contains (x:'a) (s:set<'a>) : Cost.t<bool, unit> =
+    lazy ( Set.contains x (fst s) )
+    |> Cost.C
+
+let add (x:'a) ((s, n):set<'a>) : Cost.t<set<'a>, unit> =
+    lazy (
+        if s |> Set.contains x then s, n
+        elif n <= System.UInt32.MaxValue - 1u then Set.add x s, n+1u
+        else failwith "Exceeded max set size"
+    )
+    |> Cost.C
+
+let remove (x:'a) ((s, n):set<'a>) : Cost.t<set<'a>, unit> =
+    lazy (
+        if not (s |> Set.contains x) then s, n
+        else Set.remove x s, n-1u
+    )
+    |> Cost.C
