src/Zulib/fstar/Zen.Base.fst
@@ -7,43 +7,43 @@ val const_(#a #b:Type): a -> b -> a
 let const_ #_ #_ x _ = x
 
 (** [|>] is equivalent to F#'s [|>]. *)
-unfold val ( |> ) (#a #b:Type): a -> (a->b) -> b
-unfold let ( |> ) #_ #_ x f = f x
+val ( |> ) (#a #b:Type): a -> (a->b) -> b
+let ( |> ) #_ #_ x f = f x
 
 (** [<|] is equivalent to F#'s [<|].
     Note that [<|] is left associative!
     Use [@] for right associativity. *)
-unfold val ( <| ) (#a #b:Type): (a->b) -> a -> b
-unfold let ( <| ) #_ #_ f x = f x
+val ( <| ) (#a #b:Type): (a->b) -> a -> b
+let ( <| ) #_ #_ f x = f x
 
 (** [@] is equivalent to Haskell's [$].
     Note that [@] is right associative!
     Use [<|] for left associativity. *)
-unfold val ( @ ) (#a #b:Type): (a->b) -> a -> b
-unfold let ( @ ) #_ #_ f x = f x
+val ( @ ) (#a #b:Type): (a->b) -> a -> b
+let ( @ ) #_ #_ f x = f x
 
 (** [>>] is equivalent to F#'s [>>]. *)
-unfold val ( >> ) (#a #b #c:Type): (a->b)->(b->c)->(a->c)
-unfold let ( >> ) #_ #_ #_ f g = fun x -> g (f x)
+val ( >> ) (#a #b #c:Type): (a->b)->(b->c)->(a->c)
+let ( >> ) #_ #_ #_ f g = fun x -> g (f x)
 
 (** [<<] is equivalent to F#'s [<<] or Haskell's [.].
     Note that [<<] is left associative!
     Use [@] for right associativity. *)
-unfold val ( << ) (#a #b #c:Type): (b->c)->(a->b)->(a->c)
-unfold let ( << ) #_ #_ #_ f g = fun x -> f (g x)
+val ( << ) (#a #b #c:Type): (b->c)->(a->b)->(a->c)
+let ( << ) #_ #_ #_ f g = fun x -> f (g x)
 
 (** [@<<] is equivalent to F#'s [<<] or Haskell's [.].
     Note that [@<<] is right associative!
     Use [<<] for left associativity.*)
-unfold val ( @<< ) (#a #b #c:Type): (b->c)->(a->b)->(a->c)
-unfold let ( @<< ) #_ #_ #_ f g = fun x -> f (g x)
+val ( @<< ) (#a #b #c:Type): (b->c)->(a->b)->(a->c)
+let ( @<< ) #_ #_ #_ f g = fun x -> f (g x)
 
 (** [flip] x y reverses the order of arguments. Named as in Haskell.
     [flip] is useful for writing 'pointfree' code.
     However, pointfree code is rarely useful.
     Use with caution. With great power comes great responsibility. *)
-unfold val flip(#a #b #c:Type): (a -> b -> c) -> b -> a -> c
-unfold let flip #_ #_ #_ f x y = f y x
+val flip(#a #b #c:Type): (a -> b -> c) -> b -> a -> c
+let flip #_ #_ #_ f x y = f y x
 
 (*) Robocow
 
