src/Zulib/fstar/Zen.Array.Realized.fsti
@@ -1,7 +1,6 @@
 module Zen.Array.Realized
 
 open Zen.Cost
-module M = FStar.Mul
 module V = Zen.Vector
 
 assume new type array (a:Type u#a) : nat -> Type u#a
@@ -10,7 +9,7 @@ assume Array_hasEq: forall (a:Type) (n:nat). {:pattern (hasEq (array a n))}
 
 (** init returns an array of length l for which the i-th element is f(i) *)
 val init(#a:Type)(#n:nat): l:nat -> f:(i:nat{i<l} -> cost a n)
-  -> cost (array a l) M.((l+1)*(n+1))
+  -> cost (array a l) ((l+1)*(n+1))
 
 val empty: array 'a 0
 
@@ -20,7 +19,7 @@ assume Init_elem:
   forall #a #n (l:nat) (f: i:nat{i<l} -> cost a n) (i:nat{i<l}).
   force (init l f >>= elem i) == force (f i)
 
-val ofVec(#a:Type)(#l:nat): V.t a l -> cost (array a l) M.(2*(l+1))
+val ofVec(#a:Type)(#l:nat): V.t a l -> cost (array a l) (2*(l+1))
 assume OfVec_elem:
   forall #a #l (v:V.t a l) (i:nat{i<l}).
   force (ofVec v >>= elem i) == force (V.nth v i)
