src/Zulib/fstar/Zen.Set.fsti
@@ -1,0 +1,16 @@
+module Zen.Set
+
+open Zen.Cost
+
+assume new type set : eqtype -> eqtype
+//assume Set_hasEq: forall (a:eqtype). hasEq (set a)
+
+type t (a:eqtype) = set a
+
+val nullSet (#a:eqtype): set a
+
+val contains(#a:eqtype): a -> set a -> bool `cost` 64
+
+val add(#a:eqtype): a -> set a -> set a `cost` 64
+
+val remove(#a:eqtype): a -> set a -> set a `cost` 64
