src/Zulib/fstar/Zen.TxSkeleton.fsti
@@ -3,7 +3,6 @@ module Zen.TxSkeleton
 open Zen.Cost
 open Zen.Types
 
-module M = FStar.Mul
 module V = Zen.Vector
 module U64 = FStar.UInt64
 
@@ -14,7 +13,7 @@ val addInput: pointedOutput -> txSkeleton -> txSkeleton `cost` 64
 val addInputs(#n:nat):
   pointedOutput `V.t` n
   -> txSkeleton
-  -> txSkeleton `cost` M.(64 * n + 64)
+  -> txSkeleton `cost` (64 * n + 64)
 
 val lockToContract:
   asset
@@ -54,13 +53,13 @@ val destroy:
   -> contractHash
   -> txSkeleton
   -> txSkeleton `cost` 64
-  
+
 val fromWallet(#n:nat):
   asset ->
   amount:U64.t ->
-  contractHash -> 
-  wallet n ->  
+  contractHash ->
+  wallet n ->
   txSkeleton ->
-  option txSkeleton `cost` M.(n * 128 + 192)   
+  option txSkeleton `cost` (n * 128 + 192)
 
 val isValid: txSkeleton -> bool `cost` 64
