src/Zulib/fstar/Zen.Types.Data.fst
@@ -1,10 +1,9 @@
 module Zen.Types.Data
 
+open Zen.Dictionary
 open Zen.Types.Extracted
-open Zen.Cost
 
 module A = Zen.Array
-module OT = Zen.OptionT
 //module I8  = FStar.Int8
 //module I32 = FStar.Int32
 module I64 = FStar.UInt64
@@ -16,45 +15,19 @@ type data =
     //| I8  of I8.t
     //| I32 of I32.t
     | I64 of I64.t
-    | I64Array: #l:nat -> I64.t `A.t` l -> data
+    | I64Array: (l:nat & I64.t `A.t` l) -> data
     | Byte of U8.t
-    | ByteArray: #l:nat -> U8.t `A.t` l -> data
+    | ByteArray: (l:nat & U8.t `A.t` l) -> data
     | U32 of U32.t
-    | U32Array: #l:nat -> U32.t `A.t` l -> data
+    | U32Array: (l:nat & U32.t `A.t` l) -> data
     | U64 of U64.t
-    | U64Array: #l:nat -> U64.t `A.t` l -> data
+    | U64Array: (l:nat & U64.t `A.t` l) -> data
     | String of string
-    | StringArray: #l:nat -> U64.t `A.t` l -> data
+    | StringArray: (l:nat & string `A.t` l) -> data
     | Hash of hash
-    | HashArray: #l:nat -> U64.t `A.t` l -> data
+    | HashArray: (l:nat & hash `A.t` l) -> data
     | Lock of lock
-    | LockArray: #l:nat -> U64.t `A.t` l -> data
+    | LockArray: (l:nat & lock `A.t` l) -> data
     | Tuple of (data ** data)
 
-val getI64 : data -> option I64.t `cost` 2
-let getI64 = function | I64 x -> OT.incSome 2 x
-                      | _ -> OT.incNone 2
-
-val getByte : data -> option U8.t `cost` 2
-let getByte = function | Byte b -> OT.incSome 2 b
-                       | _ -> OT.incNone 2
-
-val getU32 : data -> option U32.t `cost` 2
-let getU32 = function | U32 x -> OT.incSome 2 x
-                      | _ -> OT.incNone 2
-
-val getU64 : data -> option U64.t `cost` 2
-let getU64 = function | U64 x -> OT.incSome 2 x
-                      | _ -> OT.incNone 2
-
-val getString : data -> option string `cost` 2
-let getString = function | String s -> OT.incSome 2 s
-                         | _ -> OT.incNone 2
-
-val getHash : data -> option hash `cost` 2
-let getHash = function | Hash h -> OT.incSome 2 h
-                       | _ -> OT.incNone 2
-
-val getLock : data -> option lock `cost` 2
-let getLock = function | Lock l -> OT.incSome 2 l
-                       | _ -> OT.incNone 2
+type args = dictionary data
